finish correctness of forward_subsumption_one

Weidenbach_Book/Watched_Literals/Watched_Literals_List_Inprocessing.thy
@@ -1641,7 +1641,7 @@ definition forward_subsumption_one_pre :: \<open>nat \<Rightarrow> 'v twl_st_l \
   set (get_all_mark_of_propagated (get_trail_l S)) \<subseteq> {0} \<and>
   C \<in># dom_m (get_clauses_l S) \<and>
   (\<forall>L \<in># mset (get_clauses_l S \<propto> C). undefined_lit (get_trail_l S) L) \<and>
-  length (get_clauses_l S \<propto> C) \<ge> 2)\<close>
+  length (get_clauses_l S \<propto> C) > 2)\<close>
 
 datatype 'v subsumption =
   is_subsumed: SUBSUMED_BY (subsumed_by: nat) |
@@ -2002,11 +2002,11 @@ lemma subresolution_strengtheningI:
   done
 
 lemma subsume_or_strengthen:
-  assumes \<open>subsume_or_strengthen_pre C s (M, N, D, NE, UE, NEk, UEk, NS, US, N0, U0, WS, Q)\<close> \<open>C \<in># dom_m N\<close>
+  assumes \<open>subsume_or_strengthen_pre C s S\<close> \<open>C \<in># dom_m (get_clauses_l S)\<close>
   shows
-    \<open>subsume_or_strengthen C s (M, N, D, NE, UE, NEk, UEk, NS, US, N0, U0, WS, Q) \<le>\<Down>Id (SPEC(\<lambda>T.
-  cdcl_twl_inprocessing_l\<^sup>*\<^sup>* (M, N, D, NE, UE, NEk, UEk, NS, US, N0, U0, WS, Q) T \<and>
-    (s = NONE \<longrightarrow> T = (M, N, D, NE, UE, NEk, UEk, NS, US, N0, U0, WS, Q))))\<close>
+    \<open>subsume_or_strengthen C s S \<le>\<Down>Id (SPEC(\<lambda>T. cdcl_twl_inprocessing_l\<^sup>*\<^sup>* S T \<and>
+      (s = NONE \<longrightarrow> T = S) \<and>
+      (length (get_clauses_l S \<propto> C) > 2 \<longrightarrow> get_trail_l S = get_trail_l T)))\<close>
   using assms unfolding subsume_or_strengthen_def
   apply refine_vcg+
   subgoal by auto
@@ -2818,39 +2818,41 @@ proof -
 qed
 
 definition forward_subsumption_one_inv :: \<open>nat \<Rightarrow> 'v twl_st_l \<Rightarrow> _ \<Rightarrow> bool\<close> where
-  \<open>forward_subsumption_one_inv = (\<lambda>C S (T, xs, s).
+  \<open>forward_subsumption_one_inv = (\<lambda>C S (xs, s).
   (\<exists>S' . (S, S') \<in> twl_st_l None \<and>
       twl_struct_invs S' \<and>
       cdcl\<^sub>W_restart_mset.cdcl\<^sub>W_learned_clauses_entailed_by_init (state\<^sub>W_of S') \<and>
-    subsume_or_strengthen_pre C s T \<and>
-    C \<notin># xs \<and> C \<in># dom_m (get_clauses_l T) \<and> count_decided (get_trail_l S) = 0 \<and>
+    C \<notin># xs \<and> C \<in># dom_m (get_clauses_l S) \<and> count_decided (get_trail_l S) = 0 \<and>
     clauses_to_update_l S = {#} \<and> twl_list_invs S \<and> twl_struct_invs S' \<and>
    set (get_all_mark_of_propagated (get_trail_l S)) \<subseteq> {0} \<and>
-   cdcl\<^sub>W_restart_mset.cdcl\<^sub>W_learned_clauses_entailed_by_init (state\<^sub>W_of S') \<and>
-   cdcl_twl_inprocessing_l\<^sup>*\<^sup>* S T))\<close>
+  cdcl\<^sub>W_restart_mset.cdcl\<^sub>W_learned_clauses_entailed_by_init (state\<^sub>W_of S') \<and>
+   subsume_or_strengthen_pre C s S))\<close>
 
+definition forward_subsumption_one_select where
+  \<open>forward_subsumption_one_select C S = (\<lambda>xs. C \<notin># xs \<and>
+  (\<forall>D\<in>#xs. D \<in># dom_m (get_clauses_l S) \<longrightarrow> length (get_clauses_l S \<propto> D) > 2
+     \<and> (\<forall>L\<in> set (get_clauses_l S \<propto> D). undefined_lit (get_trail_l S) L)))\<close>
 
 definition forward_subsumption_one :: \<open> nat \<Rightarrow> 'v twl_st_l \<Rightarrow> ('v twl_st_l \<times> bool) nres\<close> where
   \<open>forward_subsumption_one = (\<lambda>C S . do {
     ASSERT(forward_subsumption_one_pre C S);
-    xs \<leftarrow> SPEC (\<lambda>xs. C \<notin># xs);
-    (S, xs, s) \<leftarrow>
-      WHILE\<^sub>T\<^bsup> forward_subsumption_one_inv C S \<^esup> (\<lambda>(S, xs, s). xs \<noteq> {#} \<and> s = NONE \<and> get_conflict_l S = None)
-      (\<lambda>(S, xs, s). do {
+    xs \<leftarrow> SPEC (forward_subsumption_one_select C S);
+    (xs, s) \<leftarrow>
+      WHILE\<^sub>T\<^bsup> forward_subsumption_one_inv C S \<^esup> (\<lambda>(xs, s). xs \<noteq> {#} \<and> s = NONE)
+      (\<lambda>(xs, s). do {
         C' \<leftarrow> SPEC(\<lambda>C'. C' \<in># xs);
         if C' \<notin># dom_m (get_clauses_l S) 
-        then RETURN (S, remove1_mset C' xs, s)
+        then RETURN (remove1_mset C' xs, s)
         else do {
-          S \<leftarrow> simplify_clause_with_unit_st C' S;
-          if C' \<notin># dom_m (get_clauses_l S) \<or> get_conflict_l S \<noteq> None
-          then RETURN (S, remove1_mset C' xs, s)
+          if C' \<notin># dom_m (get_clauses_l S)
+          then RETURN (remove1_mset C' xs, s)
           else do  {
             s \<leftarrow> SPEC(try_to_subsume C C' (get_clauses_l S));
-           RETURN (S, remove1_mset C' xs, s)
+           RETURN (remove1_mset C' xs, s)
           }
         }
       })
-      (S, xs, NONE);
+      (xs, NONE);
     S \<leftarrow> subsume_or_strengthen C s S;
     RETURN (S, s \<noteq> NONE)
   }
@@ -2864,48 +2866,14 @@ lemma subset_mset_removeAll_iff:
     mset_le_subtract_right removeAll_mset_filter_mset replicate_mset_minus_replicate_mset_same
     replicate_mset_subseteq_iff_le set_mset_minus_replicate_mset(1) subset_mset.diff_add)
 
+lemma tautology_add_subset: \<open>A \<subseteq># Aa \<Longrightarrow> tautology (A + Aa) \<longleftrightarrow> tautology Aa\<close> for A Aa
+  by (metis mset_subset_eqD subset_mset.add_diff_inverse tautology_minus tautology_union)
+(*End Move*)
 
-lemma forward_subsumption_one_inv_alt_def:
-  \<open>forward_subsumption_one_inv = (\<lambda>C S (T, xs, s).
-  (\<exists>S' T'. (S, S') \<in> twl_st_l None \<and>
-      twl_struct_invs S' \<and>
-      cdcl\<^sub>W_restart_mset.cdcl\<^sub>W_learned_clauses_entailed_by_init (state\<^sub>W_of S') \<and>
-    subsume_or_strengthen_pre C s T \<and>
-    C \<notin># xs \<and> C \<in># dom_m (get_clauses_l T) \<and> count_decided (get_trail_l S) = 0 \<and> 
-    clauses_to_update_l S = {#} \<and> twl_list_invs S \<and> twl_struct_invs S' \<and>
-   set (get_all_mark_of_propagated (get_trail_l S)) \<subseteq> {0} \<and>
-   cdcl\<^sub>W_restart_mset.cdcl\<^sub>W_learned_clauses_entailed_by_init (state\<^sub>W_of S') \<and>
-   (T, T') \<in> twl_st_l None \<and>
-      twl_struct_invs T' \<and>
-      cdcl\<^sub>W_restart_mset.cdcl\<^sub>W_learned_clauses_entailed_by_init (state\<^sub>W_of T') \<and>
-    C \<notin># xs \<and> C \<in># dom_m (get_clauses_l T) \<and> count_decided (get_trail_l T) = 0 \<and> 
-    clauses_to_update_l T = {#} \<and> twl_list_invs T \<and> twl_struct_invs T' \<and>
-   set (get_all_mark_of_propagated (get_trail_l T)) \<subseteq> {0} \<and>
-   cdcl\<^sub>W_restart_mset.cdcl\<^sub>W_learned_clauses_entailed_by_init (state\<^sub>W_of T') \<and>
-   cdcl_twl_inprocessing_l\<^sup>*\<^sup>* S T))\<close>
-  unfolding forward_subsumption_one_inv_def
-  apply (rule iffI ext)+
-  apply (case_tac x; hypsubst)
-  unfolding prod.simps
-  apply normalize_goal+
-  apply (frule rtranclp_cdcl_twl_inprocessing_l_twl_st_l; assumption?)
-  apply (rule_tac x=xa in exI)
-  apply (rule_tac x=V in exI)
-  apply (simp add: rtranclp_cdcl_twl_inprocessing_l_count_decided
-   rtranclp_cdcl_twl_inprocessing_l_clauses_to_update_l rtranclp_cdcl_twl_inprocessing_l_get_all_mark_of_propagated)
-  apply (drule rtranclp_cdcl_twl_inprocessing_l_get_all_mark_of_propagated, blast)
-  apply (case_tac x; hypsubst)
-  unfolding prod.simps
-  apply normalize_goal+
-  apply (frule rtranclp_cdcl_twl_inprocessing_l_twl_st_l; assumption?)
-  apply (rule_tac x=xa in exI)
-  apply simp
-  done
-
-(*
 lemma forward_subsumption_one:
   assumes \<open>forward_subsumption_one_pre C S\<close>
-  shows \<open>forward_subsumption_one C S \<le> \<Down>{((st, SR), st'). st = st' \<and> (\<not>SR \<longrightarrow> st = S)} (SPEC(cdcl_twl_inprocessing_l\<^sup>*\<^sup>* S))\<close>
+  shows \<open>forward_subsumption_one C S \<le> \<Down>{((st, SR), st'). st = st' \<and> (\<not>SR \<longrightarrow> st = S)}
+       (SPEC(\<lambda>T. cdcl_twl_inprocessing_l\<^sup>*\<^sup>* S T \<and> get_trail_l T = get_trail_l S))\<close>
 proof -
   obtain x where
     Sx: \<open>(S, x) \<in> twl_st_l None\<close> and
@@ -2917,102 +2885,67 @@ proof -
     clss: \<open>clauses_to_update_l S = {#}\<close> \<open>get_conflict_l S = None\<close> and
     no_annot: \<open>set (get_all_mark_of_propagated (get_trail_l S)) \<subseteq> {0}\<close> and
     init: \<open>cdcl\<^sub>W_restart_mset.cdcl\<^sub>W_learned_clauses_entailed_by_init (state\<^sub>W_of x)\<close> and
-    dec: \<open>count_decided (get_trail_l S) = 0\<close>
+    dec: \<open>count_decided (get_trail_l S) = 0\<close> and
+    undef_C: \<open>\<forall>L\<in>#mset (get_clauses_l S \<propto> C). undefined_lit (get_trail_l S) L\<close> and
+    le_C: \<open>2 < length (get_clauses_l S \<propto> C)\<close>
     using assms unfolding forward_subsumption_one_pre_def twl_struct_invs_def
       pcdcl_all_struct_invs_def state\<^sub>W_of_def
     apply -
-    by normalize_goal+ blast
-  have [refine0]: \<open>wf (measure (\<lambda>(_, d, _). size d))\<close>
+    by normalize_goal+ blast  have \<open>C \<noteq> 0\<close>
+    using list_invs C by (auto simp: twl_list_invs_def)
+  then have C_annot: \<open>C \<notin> set (get_all_mark_of_propagated (get_trail_l S))\<close>
+    using no_annot by blast
+
+  have [refine0]: \<open>wf (measure (\<lambda>(d, _). size d))\<close>
     by auto
   have H: \<open>length (get_clauses_l S \<propto> D) \<ge>2\<close> \<open>distinct (get_clauses_l S \<propto> D)\<close>  \<open>D \<noteq> 0\<close>
-    \<open>D \<notin> set (get_all_mark_of_propagated (get_trail_l S))\<close> if \<open>D \<in># dom_m (get_clauses_l S)\<close>for D
+    \<open>D \<notin> set (get_all_mark_of_propagated (get_trail_l S))\<close>
+    \<open>\<not>tautology (mset (get_clauses_l S \<propto> D))\<close>
+    if \<open>D \<in># dom_m (get_clauses_l S)\<close>for D
     using st_inv that Sx list_invs no_annot unfolding twl_struct_invs_def twl_list_invs_def apply -
     by (auto simp: twl_struct_invs_def twl_st_l_def ran_m_def conj_disj_distribR
       twl_st_inv.simps Collect_disj_eq image_image image_Un Collect_conv_if mset_take_mset_drop_mset'
       dest!: multi_member_split split: if_splits
       simp flip: insert_compr)
+
   have H2: \<open>\<not>tautology (mset (get_clauses_l S \<propto> D))\<close> if \<open>D \<in># dom_m (get_clauses_l S)\<close> for D
     using list_invs that by (auto simp: twl_list_invs_def ran_m_def)
-find_theorems simplify_clause_with_unit_st
 
-  have \<open>subsume_or_strengthen_pre C (snd (snd xb')) U\<close>
+  have forward_subsumption_one_inv: \<open>forward_subsumption_one_inv C S (remove1_mset xa aa, xb)\<close>
     if
       \<open>forward_subsumption_one_pre C S\<close> and
-      \<open>C \<notin># xs\<close> and
-      \<open>xa \<in># b\<close> and
-      \<open>xa \<in># dom_m (get_clauses_l ab)\<close> and
-      \<open>xa \<in># dom_m (get_clauses_l U) \<and> get_conflict_l U = None\<close> and
-      xb': \<open>xb'
-    \<in> (\<lambda>x. (U, remove1_mset xa b, x)) `
-      Collect (try_to_subsume C xa (get_clauses_l U))\<close> and
-      \<open>s = (ab, b, NONE)\<close> and
-      \<open>ba' = (b, NONE)\<close> and
-      \<open>b \<noteq> {#}\<close> and
-      abU: \<open>ab = U \<or> cdcl_twl_unitres_l ab U \<or> cdcl_twl_unitres_true_l ab U\<close> and
-      \<open>a = ab\<close> and
-      \<open>(S, x) \<in> twl_st_l None\<close> and
-      \<open>c = NONE\<close> and
-      \<open>get_conflict_l ab = None\<close> and
-      \<open>set (get_all_mark_of_propagated (get_trail_l U))
-    \<subseteq> insert 0 (set (get_all_mark_of_propagated (get_trail_l ab)))\<close> and
-      \<open>aa = b\<close> and
-      \<open>ba = NONE\<close> and
-      dom_U: \<open>dom_m (get_clauses_l U) = dom_m (get_clauses_l ab) \<or>
-    dom_m (get_clauses_l U) = remove1_mset xa (dom_m (get_clauses_l ab))\<close> and
-      all_undef: \<open>\<forall>L\<in>set (get_clauses_l U \<propto> xa). undefined_lit (get_trail_l U) L\<close> and
-      \<open>cdcl\<^sub>W_restart_mset.cdcl\<^sub>W_learned_clauses_entailed_by_init
-     (state_of (pstate\<^sub>W_of x))\<close> and
-      \<open>subsume_or_strengthen_pre C NONE S\<close> and
-      \<open>C \<notin># b\<close> and
-      \<open>C \<in># dom_m (get_clauses_l ab)\<close> and
-      \<open>count_decided (get_trail_l S) = 0\<close> and
-      \<open>clauses_to_update_l S = {#}\<close> and
-      \<open>twl_list_invs S\<close> and
-      \<open>twl_struct_invs x\<close> and
-      \<open>set (get_all_mark_of_propagated (get_trail_l S)) \<subseteq> {0}\<close> and
-      ST: \<open>cdcl_twl_inprocessing_l\<^sup>*\<^sup>* S ab\<close>
-    for ab U xa c xb xb' ba'
+      select: \<open>forward_subsumption_one_select C S xs\<close> and
+      inv: \<open>forward_subsumption_one_inv C S s\<close> and
+      \<open>case s of (xs, s) \<Rightarrow> xs \<noteq> {#} \<and> s = NONE\<close> and
+      st[simp]: \<open>s = (aa, ba)\<close> and
+      xa_aa: \<open>xa \<in># aa\<close> and
+      xa: \<open>\<not> xa \<notin># dom_m (get_clauses_l S)\<close> and
+      subs: \<open>try_to_subsume C xa (get_clauses_l S) xb\<close>
+    for xs s b aa ba xa xb
   proof -
-    have C_ab: \<open>C \<in># dom_m (get_clauses_l ab)\<close>
-      using that by simp_all
-    have SU: \<open>cdcl_twl_inprocessing_l\<^sup>*\<^sup>* S U\<close>
-      using ST abU by (auto dest!: cdcl_twl_inprocessing_l.intros)
-    have no_annot: \<open>set (get_all_mark_of_propagated (get_trail_l U)) \<subseteq> {0}\<close> and
-      dec: \<open>count_decided (get_trail_l U) = 0\<close>
-      using \<open>set (get_all_mark_of_propagated (get_trail_l S)) \<subseteq> {0}\<close>
-        rtranclp_cdcl_twl_inprocessing_l_get_all_mark_of_propagated[OF SU]
-        rtranclp_cdcl_twl_inprocessing_l_count_decided[OF SU]
-      unfolding \<open>count_decided (get_trail_l S) = 0\<close>
-      by blast+
-    obtain x where
-      Sx: \<open>(U, x) \<in> twl_st_l None\<close> and
-      struct: \<open>twl_struct_invs x\<close> and
-      list_invs: \<open>twl_list_invs U\<close> and
-      init: \<open>cdcl\<^sub>W_restart_mset.cdcl\<^sub>W_learned_clauses_entailed_by_init (state\<^sub>W_of x)\<close>
-      subgoal premises p
-        by (rule rtranclp_cdcl_twl_inprocessing_l_twl_st_l[OF SU Sx struct list_invs init])
-         (rule that; (assumption)?)
-      done
-    have \<open>cdcl\<^sub>W_restart_mset.cdcl\<^sub>W_all_struct_inv (state\<^sub>W_of x)\<close> and
-      st_inv: \<open>twl_st_inv x\<close>
-      using struct
-      unfolding forward_subsumption_one_pre_def twl_struct_invs_def
-        pcdcl_all_struct_invs_def state\<^sub>W_of_def by fast+
-    have C: \<open>C \<in># dom_m (get_clauses_l U)\<close>
-      using dom_U C_ab that(3,5,22) by (auto intro!: in_remove1_msetI)
-    have H: \<open>length (get_clauses_l U \<propto> D) \<ge>2\<close> \<open>distinct (get_clauses_l U \<propto> D)\<close>  \<open>D \<noteq> 0\<close>
-      \<open>D \<notin> set (get_all_mark_of_propagated (get_trail_l U))\<close> if \<open>D \<in># dom_m (get_clauses_l U)\<close>for D
-      using st_inv that Sx list_invs no_annot unfolding twl_struct_invs_def twl_list_invs_def apply -
-      by (auto simp: twl_struct_invs_def twl_st_l_def ran_m_def conj_disj_distribR
-        twl_st_inv.simps Collect_disj_eq image_image image_Un Collect_conv_if mset_take_mset_drop_mset'
-        dest!: multi_member_split split: if_splits
-        simp flip: insert_compr)
-    show ?thesis
-      using H C xb' dec all_undef unfolding subsume_or_strengthen_pre_def try_to_subsume_def
-      apply (case_tac x)
-      apply (auto split: subsumption.splits simp add: state_decomp_to_state_l) sorry
-  qed
+    have [simp]: \<open>C \<noteq> xa\<close>
+      using xa_aa select inv unfolding forward_subsumption_one_select_def forward_subsumption_one_inv_def
+      by auto
 
+    have [intro]: \<open>x21 \<in> set (get_clauses_l S \<propto> xa) \<Longrightarrow>
+    - x21 \<in> set (get_clauses_l S \<propto> C) \<Longrightarrow>
+    remove1_mset x21 (mset (get_clauses_l S \<propto> xa)) \<subseteq># remove1_mset (- x21) (mset (get_clauses_l S \<propto> C)) \<Longrightarrow>
+    tautology (mset (get_clauses_l S \<propto> xa) + mset (get_clauses_l S \<propto> C) - {#- x21, x21#}) \<Longrightarrow> False\<close> for a x21
+      using multi_member_split[of x21 \<open>mset (get_clauses_l S \<propto> xa)\<close>]
+        multi_member_split[of \<open>-x21\<close> \<open>mset (get_clauses_l S \<propto> C)\<close>] H[of C] C
+      by (auto simp: tautology_add_subset tautology_add_mset)
+
+    have \<open>subsume_or_strengthen_pre C xb S\<close>
+      using undef_C le_C dec clss C_annot subs H xa C H[of C] unfolding subsume_or_strengthen_pre_def
+      by (auto simp: try_to_subsume_def split: subsumption.splits)
+    then show ?thesis
+      using inv
+      unfolding forward_subsumption_one_inv_def prod.simps st apply -
+      apply normalize_goal+
+      apply (rule exI[of _ x])
+      apply (use Sx struct st_inv init dec in simp_all)
+      done
+  qed
   show ?thesis
     unfolding forward_subsumption_one_def conc_fun_RES
     apply (rewrite at \<open>_ \<le> \<hole>\<close> RES_SPEC_conv)
@@ -3020,104 +2953,31 @@ find_theorems simplify_clause_with_unit_st
       simplify_clause_with_unit_st_spec[THEN order_trans] if_rule)
     subgoal using assms by auto
     subgoal for ax
-      unfolding forward_subsumption_one_inv_def prod.simps
+      unfolding forward_subsumption_one_inv_def prod.simps forward_subsumption_one_select_def
       apply (rule_tac x=x in exI)
       using Sx H struct st_inv C init by (auto simp add: subsume_or_strengthen_pre_def forward_subsumption_one_pre_def)
    subgoal for xs
      unfolding simplify_clause_with_unit_st_pre_def forward_subsumption_one_inv_def case_prod_beta
-     apply normalize_goal+ 
+     apply normalize_goal+
      by (rule_tac x=x in exI)
       (auto dest: in_diffD)
    subgoal
      unfolding simplify_clause_with_unit_st_pre_def forward_subsumption_one_inv_def case_prod_beta
-     apply normalize_goal+ 
-     by  (auto dest: multi_member_split)
-   subgoal
-     unfolding simplify_clause_with_unit_st_pre_def forward_subsumption_one_inv_alt_def case_prod_beta
-     apply normalize_goal+ 
-    apply (intro conjI)
-    apply ((solves \<open>use dec init C in \<open>simp\<close>\<close>))+
-    apply ((solves \<open>use dec init C in \<open>fastforce\<close>\<close>)?)
-    done
-
-   subgoal for xs s a b aa ba xa unfolding Down_id_eq
-     apply (intro SPEC_rule)
-     apply (rule if_rule)
-     subgoal
-       apply clarsimp
-       apply (intro conjI)
-       subgoal
-         unfolding forward_subsumption_one_inv_def prod.simps
-         apply normalize_goal+
-         apply (rule_tac x=x in exI)
-         apply simp
-        apply (intro conjI)
-        defer
-        apply (metis in_diffD) 
-        apply (metis in_remove1_msetI)
-        apply (auto dest!: cdcl_twl_inprocessing_l.intros)
-        done
-     subgoal by (auto dest!: multi_member_split)
-     done
-   subgoal for U
-     unfolding RES_RETURN_RES
-     apply (subst nres_order_simps)
-     apply rule
-     apply (subst mem_Collect_eq)
-     apply (intro conjI)
-     subgoal for x
-        apply (case_tac s, hypsubst)
-         unfolding forward_subsumption_one_inv_def prod.simps case_prod_beta
-         apply normalize_goal+
-         apply (rule_tac x=x in exI)
-         apply simp
-         apply (intro conjI)
-defer
-       apply (clarsimp dest!: in_diffD)
-       apply (auto dest!: in_diffD intro: in_remove1_msetI)[]
-       apply (auto dest!: cdcl_twl_inprocessing_l.intros)[]
-explore_have
-find_theorems subsume_or_strengthen_pre 
- apply simp
-     apply rule
-     apply simp
-     apply (intro conjI impI)
      apply normalize_goal+
-    
-
-       find_theorems "SPEC _ \<le> SPEC _"
-oops
-      using H by (auto simp: subsume_or_strengthen_pre_def
-      forward_subsumption_one_pre_def distinct_mset_dom distinct_mset_remove1_All
-       forward_subsumption_one_inv_def subset_mset_removeAll_iff split)
-    subgoal 
-      unfolding simplify_clause_with_unit_st_pre_def
- sorry
-    subgoal by (auto simp: forward_subsumption_one_inv_def dest: in_diffD)
-    subgoal by (auto simp: forward_subsumption_one_inv_def dest: multi_member_split)
-    subgoal for a b aa ba ab bb ac bc ad bd ae be af bf ag bg ah bh ai bi aj bj ak bk x s al bl xa xb
-      using H C H2 not_tautology_mono[of \<open>mset (removeAll _ (get_clauses_l S \<propto> C))\<close>
-        \<open>mset (get_clauses_l S \<propto> C)\<close>]
-      apply (auto simp: try_to_subsume_def distinct_mset_dom distinct_mset_remove1_All
-        subsume_or_strengthen_pre_def subset_mset_removeAll_iff tautology_union
-        forward_subsumption_one_inv_def
-        simp del: mset_removeAll
-        simp flip: mset_removeAll
-        split: subsumption.splits
-        dest: in_diffD)[]
-       apply (metis subset_mset.diff_add tautology_union)
-       by (smt (z3) count_le_replicate_mset_subset_eq in_replicate_mset order_refl set_mset_mset subset_mset.diff_add tautology_minus union_iff)
-    subgoal
-      by (auto dest!: multi_member_split)
-    subgoal
-      unfolding forward_subsumption_one_inv_def by blast
-    subgoal unfolding forward_subsumption_one_pre_def by auto
-    subgoal using clss apply (auto simp only:)
-      sorry
-    done
+     by  (auto dest: multi_member_split)
+   subgoal by (auto simp: forward_subsumption_one_inv_def)
+   subgoal by (auto dest!: multi_member_split)
+   subgoal by (rule forward_subsumption_one_inv)
+   subgoal by (auto dest!: multi_member_split)
+   subgoal
+     unfolding forward_subsumption_one_inv_def
+     by fast
+   subgoal using C by auto
+   subgoal for x s a b xa
+     using le_C by fastforce
+   done
 qed
-  *)
- 
+
 
 definition simplify_clauses_with_unit_st_pre where
   \<open>simplify_clauses_with_unit_st_pre S \<longleftrightarrow> (\<exists>T.
@@ -3316,16 +3176,16 @@ lemma simplify_clauses_with_units_st_spec:
   subgoal unfolding simplify_clauses_with_unit_st_inv_def by auto
   done
 
-definition try_to_forward_subsume_inv :: \<open>bool \<Rightarrow> 'v twl_st_l \<Rightarrow> nat \<Rightarrow> nat \<times> bool \<times> 'v twl_st_l \<Rightarrow> bool\<close> where
-  \<open>try_to_forward_subsume_inv no_bin S0 = (\<lambda>C (i,brk,S).
+definition try_to_forward_subsume_inv :: \<open>'v twl_st_l \<Rightarrow> nat \<Rightarrow> nat \<times> bool \<times> 'v twl_st_l \<Rightarrow> bool\<close> where
+  \<open>try_to_forward_subsume_inv S0 = (\<lambda>C (i,brk,S).
   (cdcl_twl_inprocessing_l\<^sup>*\<^sup>* S0 S \<and>
   clauses_to_update_l S = {#} \<and>
   count_decided (get_trail_l S) = 0 \<and>
   set (get_all_mark_of_propagated (get_trail_l S)) \<subseteq> {0} \<and>
   (\<not>brk \<longrightarrow> (get_conflict_l S = None \<and> C \<in># dom_m (get_clauses_l S) \<and>
   (\<forall>L \<in># mset (get_clauses_l S \<propto> C). undefined_lit (get_trail_l S) L) \<and>
-  length (get_clauses_l S \<propto> C) \<ge> 2)) \<and>
-  (no_bin \<longrightarrow> get_trail_l S = get_trail_l S0)))\<close>
+  length (get_clauses_l S \<propto> C) > 2)) \<and>
+  (get_trail_l S = get_trail_l S0)))\<close>
 
 definition try_to_forward_subsume_pre :: \<open>nat \<Rightarrow> 'v twl_st_l \<Rightarrow> bool\<close> where
   \<open>try_to_forward_subsume_pre = (\<lambda>C S.
@@ -3340,13 +3200,13 @@ definition try_to_forward_subsume_pre :: \<open>nat \<Rightarrow> 'v twl_st_l \<
   set (get_all_mark_of_propagated (get_trail_l S)) \<subseteq> {0} \<and>
   C \<in># dom_m (get_clauses_l S) \<and>
   (\<forall>L \<in># mset (get_clauses_l S \<propto> C). undefined_lit (get_trail_l S) L) \<and>
-  length (get_clauses_l S \<propto> C) \<ge> 2)\<close>
+  length (get_clauses_l S \<propto> C) > 2)\<close>
 
-definition try_to_forward_subsume :: \<open>bool \<Rightarrow> nat \<Rightarrow> 'v twl_st_l \<Rightarrow> 'v twl_st_l nres\<close> where
-  \<open>try_to_forward_subsume no_bin C S = do {
+definition try_to_forward_subsume :: \<open>nat \<Rightarrow> 'v twl_st_l \<Rightarrow> 'v twl_st_l nres\<close> where
+  \<open>try_to_forward_subsume C S = do {
   ASSERT (try_to_forward_subsume_pre C S);
   n \<leftarrow> RES {_::nat. True};
-  (_, _, S) \<leftarrow> WHILE\<^sub>T\<^bsup> try_to_forward_subsume_inv no_bin S C\<^esup>
+  (_, _, S) \<leftarrow> WHILE\<^sub>T\<^bsup> try_to_forward_subsume_inv S C\<^esup>
     (\<lambda>(i, break, S). \<not>break \<and> i < n)
     (\<lambda>(i, break, S). do {
       (S, subs) \<leftarrow> forward_subsumption_one C S;
@@ -3360,7 +3220,7 @@ definition try_to_forward_subsume :: \<open>bool \<Rightarrow> nat \<Rightarrow>
 
 lemma try_to_forward_forward_subsumption_one_pre:
   \<open>try_to_forward_subsume_pre C S \<Longrightarrow>
-  try_to_forward_subsume_inv no_bin S C (a, False, ba) \<Longrightarrow> forward_subsumption_one_pre C ba\<close>
+  try_to_forward_subsume_inv S C (a, False, ba) \<Longrightarrow> forward_subsumption_one_pre C ba\<close>
   unfolding try_to_forward_subsume_inv_def forward_subsumption_one_pre_def case_prod_beta
     try_to_forward_subsume_pre_def
   apply normalize_goal+
@@ -3370,10 +3230,9 @@ lemma try_to_forward_forward_subsumption_one_pre:
   apply simp
   done
 
-(*
 lemma try_to_forward_subsume:
   assumes \<open>try_to_forward_subsume_pre C S\<close>
-  shows \<open>try_to_forward_subsume no_bin C S \<le> \<Down>Id (SPEC(cdcl_twl_inprocessing_l\<^sup>*\<^sup>* S))\<close>
+  shows \<open>try_to_forward_subsume C S \<le> \<Down>Id (SPEC(cdcl_twl_inprocessing_l\<^sup>*\<^sup>* S))\<close>
 proof -
   have wf: \<open>wf (measure (\<lambda>(i, _, _). Suc n - i))\<close> for n
     by auto
@@ -3409,8 +3268,8 @@ definition forward_subsumption_all_pre :: \<open>'v twl_st_l \<Rightarrow> bool\
 definition forward_subsumption_all_inv :: \<open>'v twl_st_l \<Rightarrow> nat multiset \<times> 'v twl_st_l \<Rightarrow> bool\<close> where
   \<open>forward_subsumption_all_inv S = (\<lambda>(xs, T). cdcl_twl_inprocessing_l\<^sup>*\<^sup>* S T \<and> xs \<subseteq># dom_m (get_clauses_l S))\<close>
 
-definition forward_subsumption_all :: \<open>bool \<Rightarrow> 'v twl_st_l \<Rightarrow> 'v twl_st_l nres\<close> where
-  \<open>forward_subsumption_all = (\<lambda>no_bin S. do {
+definition forward_subsumption_all :: \<open>'v twl_st_l \<Rightarrow> 'v twl_st_l nres\<close> where
+  \<open>forward_subsumption_all = (\<lambda>S. do {
   ASSERT (forward_subsumption_all_pre S);
   xs \<leftarrow> SPEC (\<lambda>xs. xs \<subseteq># (dom_m (get_clauses_l S)));
   (xs, S) \<leftarrow>
@@ -3422,7 +3281,7 @@ definition forward_subsumption_all :: \<open>bool \<Rightarrow> 'v twl_st_l \<Ri
        else do {
          S \<leftarrow> simplify_clause_with_unit_st C S;
          if get_conflict_l S = None \<and> C \<in># dom_m (get_clauses_l S) then do {
-           S \<leftarrow> try_to_forward_subsume no_bin C S;
+           (S, _) \<leftarrow> forward_subsumption_one C S;
            RETURN (remove1_mset C xs, S)
          }
          else RETURN (remove1_mset C xs, S)
@@ -3544,7 +3403,7 @@ proof -
       [simp]: \<open>count_decided (get_trail_l S) = 0\<close> and
       marks: \<open>set (get_all_mark_of_propagated (get_trail_l S)) \<subseteq> {0}\<close>
       using pre unfolding forward_subsumption_all_pre_def by fast
-    have [intro]: \<open>2 \<le> length (get_clauses_l U \<propto> C)\<close>
+    have [intro]: \<open>2 < length (get_clauses_l U \<propto> C)\<close>
       if
         H: \<open>(U, Va) \<in> twl_st_l None\<close> \<open>twl_struct_invs Va\<close>  \<open>C \<in># dom_m (get_clauses_l U)\<close>
       for Va C
